theories/Testing_Pre_orders/Testing_Predicate/Testing_Predicate.v
@@ -29,41 +29,41 @@ From stdpp Require Import finite gmap decidable.
 From Must Require Import ActTau gLts Bisimulation Lts_OBA Subset_Act WeakTransitions CodePurification
     StateTransitionSystems InteractionBetweenLts Convergence Termination FiniteImageLTS.
 
-Class Testing_Predicate (P A : Type) (attaboy : P -> Prop) `{gLts P A, !gLtsEq P A} := {
-    attaboy_decidable e : Decision (attaboy e);
-    attaboy_preserved_by_eq (p : P) q : attaboy p -> p ⋍ q -> attaboy q;
-    attaboy_preserved_by_lts_non_blocking_action p q η : non_blocking η -> p ⟶[η] q -> attaboy p -> attaboy q;
-    attaboy_preserved_by_lts_non_blocking_action_converse p q η : non_blocking η -> p ⟶[η] q -> attaboy q -> attaboy p;
+Class Testing_Predicate (P A : Type) (outcome : P -> Prop) `{gLts P A, !gLtsEq P A} := {
+    outcome_decidable e : Decision (outcome e);
+    outcome_preserved_by_eq (p : P) q : outcome p -> p ⋍ q -> outcome q;
+    outcome_preserved_by_lts_non_blocking_action p q η : non_blocking η -> p ⟶[η] q -> outcome p -> outcome q;
+    outcome_preserved_by_lts_non_blocking_action_converse p q η : non_blocking η -> p ⟶[η] q -> outcome q -> outcome p;
 }.
 
-#[global] Instance attaboy_dec `{Testing_Predicate P A attaboy} e : Decision (attaboy e).
-Proof. eapply attaboy_decidable. Defined.
+#[global] Instance outcome_dec `{Testing_Predicate P A outcome} e : Decision (outcome e).
+Proof. eapply outcome_decidable. Defined.
 
-Lemma unattaboy_preserved_by_eq `{gLtsEq P A, !Testing_Predicate P A attaboy} p q :
-  ~ attaboy p -> q ⋍ p -> ~ attaboy q.
+Lemma unoutcome_preserved_by_eq `{gLtsEq P A, !Testing_Predicate P A outcome} p q :
+  ~ outcome p -> q ⋍ p -> ~ outcome q.
 Proof.
   intros not_happy eq. intro happy.
-  eapply attaboy_preserved_by_eq in happy; eauto with mdb.
+  eapply outcome_preserved_by_eq in happy; eauto with mdb.
 Qed.
 
-Lemma unattaboy_preserved_by_lts_non_blocking_action `{gLtsEq P A, !Testing_Predicate P A attaboy} p q η :
-  non_blocking η -> p ⟶[η] q -> ~ attaboy p -> ~ attaboy q.
+Lemma unoutcome_preserved_by_lts_non_blocking_action `{gLtsEq P A, !Testing_Predicate P A outcome} p q η :
+  non_blocking η -> p ⟶[η] q -> ~ outcome p -> ~ outcome q.
 Proof.
   intros nb l1 hp hq.
-  eapply hp. eapply attaboy_preserved_by_lts_non_blocking_action_converse; eauto with mdb.
+  eapply hp. eapply outcome_preserved_by_lts_non_blocking_action_converse; eauto with mdb.
 Qed.
 
-Lemma unattaboy_preserved_by_lts_non_blocking_action_converse `{gLtsEq P A, !Testing_Predicate P A attaboy} p q η :
-  non_blocking η -> p ⟶[η] q -> ~ attaboy q -> ~ attaboy p.
+Lemma unoutcome_preserved_by_lts_non_blocking_action_converse `{gLtsEq P A, !Testing_Predicate P A outcome} p q η :
+  non_blocking η -> p ⟶[η] q -> ~ outcome q -> ~ outcome p.
 Proof.
   intros nb l1 hp hq.
-  eapply hp. eapply attaboy_preserved_by_lts_non_blocking_action; eauto with mdb.
+  eapply hp. eapply outcome_preserved_by_lts_non_blocking_action; eauto with mdb.
 Qed.
 
-Lemma unattaboy_preserved_by_wt_non_blocking_action 
-  `{gLtsOba P A, !Testing_Predicate P A attaboy} 
+Lemma unoutcome_preserved_by_wt_non_blocking_action 
+  `{gLtsOba P A, !Testing_Predicate P A outcome} 
   r1 r2 s :
-  Forall non_blocking s -> r1 ↛ -> ~ attaboy r1 -> r1 ⟹[s] r2 -> ~ attaboy r2.
+  Forall non_blocking s -> r1 ↛ -> ~ outcome r1 -> r1 ⟹[s] r2 -> ~ outcome r2.
 Proof.
   intros s_spec hst hng hw.
   induction hw; eauto.
@@ -72,26 +72,26 @@ Proof.
     inversion s_spec; subst.
     eapply IHhw. eassumption.
     eapply refuses_tau_preserved_by_lts_non_blocking_action; eauto.
-    eapply unattaboy_preserved_by_lts_non_blocking_action; eauto.
+    eapply unoutcome_preserved_by_lts_non_blocking_action; eauto.
 Qed.
 
-Lemma woutpout_preserves_attaboy `{gLtsOba P A, !Testing_Predicate P A attaboy} e m e':
-  attaboy e -> e ⟿{m} e'
-    -> attaboy e'.
+Lemma woutpout_preserves_outcome `{gLtsOba P A, !Testing_Predicate P A outcome} e m e':
+  outcome e -> e ⟿{m} e'
+    -> outcome e'.
 Proof.
   intros happy stripped.
   induction stripped.
-  + eapply attaboy_preserved_by_eq; eauto.
-  + eapply IHstripped. eapply attaboy_preserved_by_lts_non_blocking_action; eauto.
+  + eapply outcome_preserved_by_eq; eauto.
+  + eapply IHstripped. eapply outcome_preserved_by_lts_non_blocking_action; eauto.
 Qed.
 
-Lemma woutpout_preserves_attaboy_converse `{gLtsOba P A, !Testing_Predicate P A attaboy} e m e':
-  attaboy e' -> e ⟿{m} e'
-    -> attaboy e.
+Lemma woutpout_preserves_outcome_converse `{gLtsOba P A, !Testing_Predicate P A outcome} e m e':
+  outcome e' -> e ⟿{m} e'
+    -> outcome e.
 Proof.
   intros happy stripped. induction stripped.
-  + symmetry in eq. eapply attaboy_preserved_by_eq; eauto.
-  + eapply attaboy_preserved_by_lts_non_blocking_action_converse. eassumption. eassumption.
+  + symmetry in eq. eapply outcome_preserved_by_eq; eauto.
+  + eapply outcome_preserved_by_lts_non_blocking_action_converse. eassumption. eassumption.
     now eapply IHstripped.
 Qed.
 
