theories/Testing_Pre_orders/May/LiftMay.v
@@ -33,7 +33,7 @@ From Must Require Import ActTau.
 
 Lemma may_non_blocking_action_swap_l_fw_eq `{
   @gLtsObaFW P A H gLtsP gLtsEqP gLtsObaP, 
-  @gLtsObaFB T A H gLtsT gLtsEqT gLtsObaT, !Testing_Predicate T A attaboy}
+  @gLtsObaFB T A H gLtsT gLtsEqT gLtsObaT, !Testing_Predicate T A outcome}
 
   `{@Prop_of_Inter P T A parallel_inter H gLtsP gLtsT}
 
@@ -46,7 +46,7 @@ Admitted.
 
 Lemma may_non_blocking_action_swap_r_fw_eq`{
   @gLtsObaFW P A H gLtsP gLtsEqP gLtsObaP, 
-  @gLtsObaFB T A H gLtsT gLtsEqT gLtsObaT, !Testing_Predicate T A attaboy}
+  @gLtsObaFB T A H gLtsT gLtsEqT gLtsObaT, !Testing_Predicate T A outcome}
 
   `{@Prop_of_Inter P T A parallel_inter H gLtsP gLtsT}
 
@@ -59,7 +59,7 @@ Admitted.
 
 Lemma may_non_blocking_action_swap_l_fw `{
   @gLtsObaFW P A H gLtsP gLtsEqP gLtsObaP, 
-  @gLtsObaFB T A H gLtsT gLtsEqT gLtsObaT, !Testing_Predicate T A attaboy}
+  @gLtsObaFB T A H gLtsT gLtsEqT gLtsObaT, !Testing_Predicate T A outcome}
 
   `{@Prop_of_Inter P T A parallel_inter H gLtsP gLtsT}
 
@@ -72,7 +72,7 @@ Qed.
 
 Lemma may_non_blocking_action_swap_r_fw `{
   @gLtsObaFW P A H gLtsP gLtsEqP gLtsObaP, 
-  @gLtsObaFB T A H gLtsT gLtsEqT gLtsObaT, !Testing_Predicate T A attaboy}
+  @gLtsObaFB T A H gLtsT gLtsEqT gLtsObaT, !Testing_Predicate T A outcome}
 
   `{@Prop_of_Inter P T A parallel_inter H gLtsP gLtsT}
 
@@ -86,7 +86,7 @@ Qed.
 
 Lemma nf_may_fw_l `{
   @gLtsObaFB P A H gLtsP gLtsEqP gLtsObaP, !FiniteImagegLts P A,
-  @gLtsObaFB T A H gLtsT gLtsEqT gLtsObaT, !Testing_Predicate T A attaboy}
+  @gLtsObaFB T A H gLtsT gLtsEqT gLtsObaT, !Testing_Predicate T A outcome}
 
   `{@Prop_of_Inter P (mb A) A fw_inter H gLtsP MbgLts}
   `{@Prop_of_Inter (P * mb A) T A parallel_inter H (inter_lts fw_inter) gLtsT}
@@ -115,7 +115,7 @@ Qed.
 
 Lemma nf_may_fw_r `{
   @gLtsObaFB P A H gLtsP gLtsEqP gLtsObaP, !FiniteImagegLts P A ,
-  @gLtsObaFB T A H gLtsT gLtsEqT gLtsObaT, !Testing_Predicate T A attaboy}
+  @gLtsObaFB T A H gLtsT gLtsEqT gLtsObaT, !Testing_Predicate T A outcome}
 
   `{@Prop_of_Inter P (mb A) A fw_inter H gLtsP MbgLts}
   `{@Prop_of_Inter (P * mb A) T A parallel_inter H (inter_lts fw_inter) gLtsT}
@@ -135,7 +135,7 @@ Admitted.
 
 Lemma nf_may_fw `{
   @gLtsObaFB P A H gLtsP gLtsEqP gLtsObaP, !FiniteImagegLts P A ,
-  @gLtsObaFB T A H gLtsT gLtsEqT gLtsObaT, !Testing_Predicate T A attaboy}
+  @gLtsObaFB T A H gLtsT gLtsEqT gLtsObaT, !Testing_Predicate T A outcome}
 
   `{@Prop_of_Inter P (mb A) A fw_inter H gLtsP MbgLts}
   `{@Prop_of_Inter (P * mb A) T A parallel_inter H (inter_lts fw_inter) gLtsT}
@@ -150,7 +150,7 @@ Qed.
 
 Lemma may_to_may_fw `{
   @gLtsObaFB P A H gLtsP gLtsEqP gLtsObaP, !FiniteImagegLts P A,
-  @gLtsObaFB T A H gLtsT gLtsEqT gLtsObaT, !Testing_Predicate T A attaboy}
+  @gLtsObaFB T A H gLtsT gLtsEqT gLtsObaT, !Testing_Predicate T A outcome}
 
   `{@Prop_of_Inter P (mb A) A fw_inter H gLtsP MbgLts}
   `{@Prop_of_Inter (P * mb A) T A parallel_inter H (inter_lts fw_inter) gLtsT}
@@ -170,7 +170,7 @@ Admitted.
 
 Lemma may_fw_to_may `{
   @gLtsObaFB P A H gLtsP gLtsEqP gLtsObaP, !FiniteImagegLts P A,
-  @gLtsObaFB T A H gLtsT gLtsEqT gLtsObaT, !Testing_Predicate T A attaboy}
+  @gLtsObaFB T A H gLtsT gLtsEqT gLtsObaT, !Testing_Predicate T A outcome}
 
   `{@Prop_of_Inter P (mb A) A fw_inter H gLtsP MbgLts}
   `{@Prop_of_Inter (P * mb A) T A parallel_inter H (inter_lts fw_inter) gLtsT}
@@ -188,7 +188,7 @@ Admitted.
 
 Lemma may_iff_may_fw `{
   @gLtsObaFB P A H gLtsP gLtsEqP gLtsObaP, !FiniteImagegLts P A,
-  @gLtsObaFB T A H gLtsT gLtsEqT gLtsObaT, !Testing_Predicate T A attaboy}
+  @gLtsObaFB T A H gLtsT gLtsEqT gLtsObaT, !Testing_Predicate T A outcome}
 
   `{@Prop_of_Inter P (mb A) A fw_inter H gLtsP MbgLts}
   `{@Prop_of_Inter (P * mb A) T A parallel_inter H (inter_lts fw_inter) gLtsT}
@@ -208,7 +208,7 @@ Qed.
 Lemma lift_fw_ctx_pre `{
     @gLtsObaFB P A H gLtsP gLtsEqP gLtsObaP, !FiniteImagegLts P A,
     @gLtsObaFB Q A H gLtsQ gLtsEqQ gLtsObaQ, !FiniteImagegLts Q A,
-    @gLtsObaFB T A H gLtsT gLtsEqT gLtsObaT, !Testing_Predicate T A attaboy}
+    @gLtsObaFB T A H gLtsT gLtsEqT gLtsObaT, !Testing_Predicate T A outcome}
 
   `{@Prop_of_Inter P (mb A) A fw_inter H gLtsP MbgLts}
 
